Retire exh flag, finish semantics link
The various set_globals esgc etc properties remain to be done

compiler/backend/flat_patternScript.sml
@@ -17,9 +17,14 @@ val _ = Datatype `config =
   <| pat_heuristic : pattern_matching$branch list -> num ;
     type_map : (num # num) list spt |>`;
 
+Definition init_type_map_def:
+  init_type_map = sptree$fromAList
+    [(bool_id, [(0 : num, 0 : num); (1, 0)]);
+        (1 (* list_id *), [(0, 0); (0, 2)])]
+End
+
 Definition init_config_def:
-  init_config = <| pat_heuristic := K 0; type_map := sptree$fromAList
-    [(bool_id, [(0, 0); (1, 0)]); (1 (* list_id *), [(0, 0); (0, 2)])] |>
+  init_config ph = <| pat_heuristic := ph; type_map := init_type_map |>
 End
 
 Definition sum_string_ords_def:
