compiler/backend/semantics/flatPropsScript.sml
@@ -356,7 +356,6 @@ QED
 Theorem do_app_state_unchanged:
   !c s op vs s' r. do_app c s op vs = SOME (s', r) ⇒
      s.c = s'.c ∧
-     s.exh_pat = s'.exh_pat ∧
      s.check_ctor = s'.check_ctor
 Proof
   rw [do_app_cases] >>
@@ -367,7 +366,6 @@ QED
 Theorem evaluate_state_unchanged:
   (!env (s:'ffi state) e s' r. evaluate env s e = (s', r) ⇒
      s.c = s'.c ∧
-     s.exh_pat = s'.exh_pat ∧
      s.check_ctor = s'.check_ctor)
 Proof
   ho_match_mp_tac evaluate_ind >>
@@ -380,7 +378,6 @@ QED
 
 Theorem evaluate_dec_state_unchanged:
   !(s:'ffi state) d s' r. evaluate_dec s d = (s', r) ⇒
-     s.exh_pat = s'.exh_pat ∧
      s.check_ctor = s'.check_ctor
 Proof
   Cases_on `d` >> rw [evaluate_dec_def] >>
@@ -390,7 +387,6 @@ QED
 
 Theorem evaluate_decs_state_unchanged:
   !(s:'ffi state) ds s' r. evaluate_decs s ds = (s', r) ⇒
-     s.exh_pat = s'.exh_pat ∧
      s.check_ctor = s'.check_ctor
 Proof
   Induct_on `ds` >> rw [evaluate_decs_def] >>
@@ -1060,16 +1056,16 @@ QED
 
 val evaluate_decs_add_to_clock_initial_state = Q.prove(
   `r ≠ SOME (Rabort Rtimeout_error) ∧
-   evaluate_decs (initial_state ffi k x y) decs = (s',r) ⇒
-   evaluate_decs (initial_state ffi (ck + k) x y) decs =
+   evaluate_decs (initial_state ffi k x) decs = (s',r) ⇒
+   evaluate_decs (initial_state ffi (ck + k) x) decs =
    (s' with clock := s'.clock + ck,r)`,
   rw [initial_state_def]
   \\ imp_res_tac evaluate_decs_add_to_clock \\ fs []);
 
 val evaluate_decs_add_to_clock_initial_state_io_events_mono = Q.prove (
-  `evaluate_decs (initial_state ffi k x y) prog = (s',r) ==>
+  `evaluate_decs (initial_state ffi k x) prog = (s',r) ==>
    s'.ffi.io_events ≼
-   (FST (evaluate_decs (initial_state ffi (k+ck) x y) prog)).ffi.io_events`,
+   (FST (evaluate_decs (initial_state ffi (k+ck) x) prog)).ffi.io_events`,
   rw [initial_state_def]
   \\ qmatch_assum_abbrev_tac `evaluate_decs s1 _ = _`
   \\ qispl_then
@@ -1078,8 +1074,8 @@ val evaluate_decs_add_to_clock_initial_state_io_events_mono = Q.prove (
   \\ fs [Abbr`s1`]);
 
 val initial_state_with_clock = Q.prove (
-  `(initial_state ffi k x y with clock := (initial_state ffi k x y).clock + ck) =
-   initial_state ffi (k + ck) x y`,
+  `(initial_state ffi k x with clock := (initial_state ffi k x).clock + ck) =
+   initial_state ffi (k + ck) x`,
   rw [initial_state_def]);
 
 val SND_SND_lemma = prove(
@@ -1087,15 +1083,15 @@ val SND_SND_lemma = prove(
   PairCases_on `x` \\ fs []);
 
 val eval_sim_def = Define `
-  eval_sim ffi exh1 ctor1 ds1 exh2 ctor2 ds2 rel allow_fail =
+  eval_sim ffi ctor1 ds1 ctor2 ds2 rel allow_fail =
     !k res1 s2.
-      evaluate_decs (initial_state ffi k exh1 ctor1) ds1 =
+      evaluate_decs (initial_state ffi k ctor1) ds1 =
         (s2, res1) /\
       (allow_fail \/ res1 <> SOME (Rabort Rtype_error)) /\
       rel ds1 ds2
       ==>
       ?ck res2 t2.
-        evaluate_decs (initial_state ffi (k + ck) exh2 ctor2) ds2 =
+        evaluate_decs (initial_state ffi (k + ck) ctor2) ds2 =
           (t2, res2) /\
         s2.ffi = t2.ffi /\
         (res1 = NONE ==> res2 = NONE) /\
@@ -1103,11 +1099,11 @@ val eval_sim_def = Define `
         (!a. res1 = SOME (Rabort a) ==> res2 = SOME (Rabort a))`;
 
 Theorem IMP_semantics_eq:
-   eval_sim ffi exh1 ctor1 ds1 exh2 ctor2 ds2 rel F /\
-   semantics exh1 ctor1 (ffi:'ffi ffi_state) ds1 <> Fail ==>
+   eval_sim ffi ctor1 ds1 ctor2 ds2 rel F /\
+   semantics ctor1 (ffi:'ffi ffi_state) ds1 <> Fail ==>
    rel ds1 ds2 ==>
-   semantics exh1 ctor1 ffi ds1 =
-   semantics exh2 ctor2 ffi ds2
+   semantics ctor1 ffi ds1 =
+   semantics ctor2 ffi ds2
 Proof
   rewrite_tac [GSYM AND_IMP_INTRO]
   \\ strip_tac
@@ -1121,7 +1117,7 @@ Proof
     \\ IF_CASES_TAC \\ fs [SND_SND_lemma]
     \\ DEEP_INTRO_TAC some_intro \\ fs [] \\ rw []
     \\ fs [eval_sim_def]
-    \\ Cases_on `evaluate_decs (initial_state ffi k' exh1 ctor1) ds1`
+    \\ Cases_on `evaluate_decs (initial_state ffi k' ctor1) ds1`
     \\ `r' <> SOME (Rabort Rtype_error)` by metis_tac []
     \\ last_x_assum drule \\ strip_tac \\ rfs [])
   \\ DEEP_INTRO_TAC some_intro \\ fs [] \\ rw []
@@ -1168,7 +1164,7 @@ Proof
   \\ simp [Once semantics_def]
   \\ IF_CASES_TAC \\ fs [SND_SND_lemma]
   >-
-   (Cases_on `evaluate_decs (initial_state ffi k exh1 ctor1) ds1`
+   (Cases_on `evaluate_decs (initial_state ffi k ctor1) ds1`
     \\ first_x_assum (qspec_then `k` mp_tac)
     \\ disch_then (qspec_then `q` mp_tac)
     \\ disch_then (qspec_then `r` mp_tac)
@@ -1184,7 +1180,7 @@ Proof
   \\ DEEP_INTRO_TAC some_intro
   \\ fs [] \\ rw []
   >-
-   (Cases_on `evaluate_decs (initial_state ffi k exh1 ctor1) ds1`
+   (Cases_on `evaluate_decs (initial_state ffi k ctor1) ds1`
     \\ last_x_assum (qspecl_then [`k`, `q`, `r'`] mp_tac)
     \\ strip_tac \\ rfs []
     \\ fs [eval_sim_def]
@@ -1219,7 +1215,7 @@ Proof
   \\ unabbrev_all_tac \\ simp [PULL_EXISTS]
   \\ simp [LNTH_fromList, PULL_EXISTS, GSYM FORALL_AND_THM]
   \\ rpt gen_tac
-  \\ Cases_on `evaluate_decs (initial_state ffi k exh1 ctor1) ds1`
+  \\ Cases_on `evaluate_decs (initial_state ffi k ctor1) ds1`
   \\ fs [eval_sim_def]
   \\ first_x_assum drule
   \\ impl_keep_tac >- metis_tac []
@@ -1316,8 +1312,8 @@ val dest_Dlet_def = Define `dest_Dlet (Dlet e) = e`;
 val _ = export_rewrites ["is_Dlet_def", "dest_Dlet_def"];
 
 Theorem initial_state_clock:
-  (initial_state ffi k b1 b2).clock = k /\
-  ((initial_state ffi k b1 b2 with clock := k1) = initial_state ffi k1 b1 b2)
+  (initial_state ffi k b1).clock = k /\
+  ((initial_state ffi k b1 with clock := k1) = initial_state ffi k1 b1)
 Proof
   EVAL_TAC
 QED
